{-# OPTIONS --postfix-projections #-}
module ChangeCat where

open import Cat
open import Prelude
open import TreeSet
open import Changes
open import Monads
open import Tones

-- There is a very simple pattern that comes up in many change functions, where
-- the derivative is "boring" - it's the same as the function itself, but
-- operating on the deltas. (The proof that it is a correct derivative is
-- usually simple as well, but I haven't found a strict pattern that it obeys.)
-- See the definition of boring-cfun, below.
--
-- We can in principle capture the type of this pattern, but the result is
-- ludicrously complicated:

-- boring-cfun : âˆ€ {j}{I : Set j} {F G : I -> Proset}
--             -> (f : âˆ€{i : I} -> F i â‡’ G i)
--             -> âˆ€ {A Î”A B Î”B : I} {PA PB}
--             -> (âˆ€{da a b} -> PA da a b -> PB (ap f da) (ap f a) (ap f b))
--             -> âˆ€{d1 d2}
--             -> ChangeFun (Change: {{F A}} (F Î”A) PA d1)
--                          (Change: {{G A}} (G Î”A) PB d2)
-- boring-cfun f x = cfun f (Ï€â‚‚ â€¢ f) x -- ========== <-- the pattern ==========

-- Moreover, it's impossible to *use* boring-cfun without explicitly providing
-- some of its many implicit arguments, which destroys any concision one might
-- hope to gain. I note this here because it's a clear instance of types, even
-- dependent types, not being powerful enough to allow even a very obvious
-- refactoring without more pain than it's worth.

 -- Category of changes
instance
  changes : Cat _ _
  Obj changes = Change
  Hom changes = ChangeFun
  ident changes = cfun id Ï€â‚‚ id
  compo changes F@(cfun f df fok) (cfun g dg gok) =
    cfun (f â€¢ g) (func&deriv F â€¢ dg) (fok â€¢ gok)

  change-products : Products changes
  change-products .top = âŠ¤-change , cfun â‰¤âŠ¤ â‰¤âŠ¤ (Î» _ â†’ TT)
  change-products .glb a b .aâˆ§b = changeÃ— a b
  change-products .glb a b .âˆ§Eâ‚ = cfun Ï€â‚ (Ï€â‚‚ â€¢ Ï€â‚) Ï€â‚
  change-products .glb a b .âˆ§Eâ‚‚ = cfun Ï€â‚‚ (Ï€â‚‚ â€¢ Ï€â‚‚) Ï€â‚‚
  change-products .glb a b .âˆ§I (cfun f df fok) (cfun g dg gok) =
    cfun âŸ¨ f , g âŸ© âŸ¨ df , dg âŸ© âŸ¨ fok , gok âŸ©

  change-sums : Sums changes
  bottom change-sums = âŠ¥-change , cfun âŠ¥â‰¤ (Ï€â‚ â€¢ Fun: âŠ¥â‰¤ Î» { {()} }) Î» { {_} {()} }
  lub change-sums a b .aâˆ¨b = change+ a b
  lub change-sums a b .âˆ¨Iâ‚ = cfun inâ‚ (Ï€â‚‚ â€¢ inâ‚) relâ‚
  lub change-sums a b .âˆ¨Iâ‚‚ = cfun inâ‚‚ (Ï€â‚‚ â€¢ inâ‚‚) relâ‚‚
  lub change-sums a b .âˆ¨E f g .funct = [ funct f , funct g ]
  lub change-sums a b .âˆ¨E {C} f g .deriv
    = uncurry (iso/âˆ¨ â€¢ [ flip [ use f , fail ] , flip [ fail , use g ] ])
    where use : âˆ€{A} -> A â‰¤ C -> ğ‘« A â‡’ iso (ğ‘¶ A) â‡¨ ğ‘« C
          use f = curry (swap â€¢ deriv f)
          fail : âˆ€{A B} -> A â‰¤ B â‡¨ (ğ‘« C)
          fail = curry (constant (dummy C))
  lub change-sums a b .âˆ¨E f g .is-id (relâ‚ da) = is-id f da
  lub change-sums a b .âˆ¨E f g .is-id (relâ‚‚ db) = is-id g db

  change-cc : CC changes
  CC.products change-cc = change-products
  _â‡¨_ {{change-cc}} = changeâ†’
  -- apply {{change-cc}} .funct = apply
  -- apply {{change-cc}} .deriv .ap ((f , a) , df , da) = ap df (a , da)
  -- apply {{change-cc}} .is-id (df:fâ†’g , dx:xâ†’y) = df:fâ†’g dx:xâ†’y
  -- curry {{change-cc}} (cfun f df ok) =
  --   cfun (curry f) (curry (isojuggle â€¢ df)) (Î» da db â†’ ok (da , db))
  apply {{change-cc}} .funct = apply
  apply {{change-cc}} .deriv .ap ((f , a) , df , da) = ap df (a , da)
  -- apply {{change-cc}} .deriv .map (faâ‰ˆgb , dfâ‰¤ , daâ‰¤) = dfâ‰¤ (juggle faâ‰ˆgb .projâ‚‚ , daâ‰¤)
  apply {{change-cc}} .deriv .map {_} {(g , b) , (dg , db)} (faâ‰ˆgb , dfâ‰¤dg , daâ‰¤db) = dfâ‰¤dg â€¢ map dg (juggle faâ‰ˆgb .projâ‚‚ , daâ‰¤db)
  apply {{change-cc}} .is-id (df:fâ†’g , dx:xâ†’y) = df:fâ†’g dx:xâ†’y
  curry {{change-cc}} (cfun f df ok) =
    cfun (curry f) (curry (isojuggle â€¢ df)) (Î» da db â†’ ok (da , db))

  change-Î  : SetÎ  zero changes
  SetÎ .Î  change-Î  = changeÎ 
  SetÎ .Î i change-Î  Î“â†’P .funct = Î i Î» a â†’ Î“â†’P a .funct
  SetÎ .Î i change-Î  Î“â†’P .deriv = Î i Î» a â†’ Î“â†’P a .deriv
  SetÎ .Î i change-Î  Î“â†’P .is-id df:fâ†’g a = Î“â†’P a .is-id df:fâ†’g
  SetÎ .Î e change-Î  a = cfun (Î e a) (Ï€â‚‚ â€¢ Î e a) (Î» df-ok â†’ df-ok a)

 -- Showing that â–¡ is a comonad on the category of changes.
Changeâ–¡ : changes â‰¤ changes
ap  Changeâ–¡ = changeâ–¡
map Changeâ–¡ (cfun f df ok) =
  cfun (map Iso f) (âˆ§/iso â€¢ map Iso df) (mapâˆ§ ok (map Iso f .map))

instance
  Changeâ–¡-comonad : Comonad Changeâ–¡
  Comonad.dup Changeâ–¡-comonad .funct = dup Iso
  Comonad.dup Changeâ–¡-comonad .deriv = Ï€â‚‚ â€¢ dup Iso
  -- agh.
  Comonad.dup Changeâ–¡-comonad .is-id p@(da:aâ†’b , aâ‰ˆb) = p , aâ‰ˆb , swap {{sets}} aâ‰ˆb
  Comonad.extract Changeâ–¡-comonad = cfun (extract Iso) (Ï€â‚‚ â€¢ extract Iso) projâ‚


-- Antisymmetry
antisymâ–¡â‰¤ : âˆ€{A B C : Change} -> Antisymmetric _â‰¡_ (ğ‘¶ A .Hom)
          -> (ğ‘¶ A .Obj -> B â‰¤ C) -> changeâ–¡ A â‰¤ B â‡¨ C
antisymâ–¡â‰¤ antisym f .funct = antisymâ‡’ antisym (Î» a â†’ f a .funct)
antisymâ–¡â‰¤ antisym f .deriv = Ï€â‚ â€¢ antisymâ‡’ (Î» xâ‰ˆy yâ‰ˆx â†’ uncurry antisym xâ‰ˆy) (Î» a â†’ f a .deriv)
antisymâ–¡â‰¤ antisym f .is-id (da , aâ‰ˆa') with uncurry antisym aâ‰ˆa'
... | refl = f _ .is-id
