\begin{figure}
  \begin{align*}
    \vals{\prod_{i} A_i} &= \prod_{i} \vals A_i &
    (x_i)_i \upd (\dx_i)_i &= (x_i \upd \dx_i)_i
    \quad\text{when defined}
    \\[1ex]
    \chgs{\prod_{i} A_i} &= \prod_{i} \chgs A_i &
    %% (x_i)_i \changeto (y_i)_i = (x_i \changeto y_i)_i
    (\dx_i)_i \compose (\dy_i)_i &= (\dx_i \compose \dy_i)_i
    \\[1ex]
    \vals{\sum_{i} A_i} &= \sum_{i} \vals A_i &
    \inj i x \upd \inj i \dx &= \inj i (x \upd \dx) \quad\text{when defined}
    \\
    \chgs{\sum_{i} A_i} &= \sum_{i} \chgs A_i &
    \inj i \dx \compose \inj j \dy &=
    \begin{cases}
      \inj i (\dx \compose \dy) & \text{if}~i=j\\
      \inj i \dx & \text{otherwise}
    \end{cases}
  \end{align*}

  \begin{align*}
    \deriv\pi_i \<x \<\dx &= \prj i \dx &
    \deriv{\fork{f_i}_i} &= \fork{\deriv f_i}_i &
    \deriv\injc_i \<x \<\dx &= \inj i \dx
  \end{align*}

  \begin{equation*}
    \deriv{\krof{f_i}_i} \<(\inj i x) \<(\inj j \dx)
    =
    \begin{cases}
      \deriv f_i \<x \<\dx & \text{if}~i = j\\
      \deriv f_i \<x \<\zero_x & \text{otherwise}
    \end{cases}
  \end{equation*}
  \vspace{-1em}

  \caption{Products and sums in \CP}
  \label{fig:CP-cartesian}
\end{figure}
